common/ListMonadFacts.v
@@ -1,25 +1,52 @@
 (** * Facts about List Monad Functions *)
 
+Require Import String.
 Require Import common.Coqlib.
+Require Import common.ListPlus.
 Require Import common.StateAndErrorMonad.
 Require Import common.StateAndErrorMonadTactics.
 Require Import common.ListMonad.
 
-Functional Scheme getv_ind := Induction for getv Sort Prop.
+(** ** Facts about [getv] *)
 
-Lemma getv_inv_state :
-  forall {state A B : Type} {eqk}
-         {eqk_dec : forall x y, {eqk x y} + {~eqk x y}}
-         {x : A} {l : list (A * B)} {s : state} {v s'},
-    getv eqk_dec x l s = OK v s' ->
-    s = s'.
-Proof.
-  intros until s.
-  functional induction (@getv state A B eqk eqk_dec x l) using getv_ind;
-    intros v s' e; (try monadInv e; auto || eapply IHm; eauto).
-Qed.
+Section GetV.
 
-Hint Resolve getv_inv_state : listmonad.
+  Functional Scheme getv_ind := Induction for getv Sort Prop.
+
+  Lemma getv_inv_state :
+    forall {state A B : Type} {eqk}
+           {eqk_dec : forall x y, {eqk x y} + {~eqk x y}}
+           {x : A} {l : list (A * B)} {s : state} {v s'},
+      getv eqk_dec x l s = OK v s' ->
+      s = s'.
+  Proof.
+    intros until s.
+    functional induction (@getv state A B eqk eqk_dec x l) using getv_ind;
+      intros v s' e; (try monadInv e; auto || eapply IHm; eauto).
+  Qed.
+
+  Hint Resolve getv_inv_state : listmonad.
+
+  Lemma getv_compl :
+    forall {state A B : Type} {l : list (A * B)}
+           {eqk} {eqk_dec : forall x y, {eqk x y} + {~eqk x y}}
+           {x : A} {s : state} {v},
+      let eqkv := fun x y => eqk (fst x) (fst y) /\ snd x = snd y in
+      InA eqkv (x, v) l ->
+      NoDupA eqk (fs l) ->
+      getv eqk_dec x l s = OK v s.
+  Proof.
+    induction l; try (solve [inversion 1]).
+    (* IND. CASE *)
+    simpl; destruct a; do 3 intro; destruct (eqk_dec x a).
+    inversion_clear 1.
+    destruct H0 as (eqk_, eq_); simpl in eq_; rewrite eq_.
+    unfold Ret; reflexivity.
+  Admitted.
+  
+End GetV.
+
+(** ** Facts about [foldl] *)
 
 Remark foldl_inv_state :
   forall {state A B : Type} {f : B -> A -> Mon B} {l b0} {s : state} {v s'}
